@prefix owl: <http://www.w3.org/2002/07/owl#> .
@prefix rdfs: <http://www.w3.org/2000/01/rdf-schema#> .
@prefix dcog: <https://datachemist.net/ontology/dcog#> .
@prefix xsd: <http://www.w3.org/2001/XMLSchema#> .

<https://datachemist.net/ontology/dcog>
  a owl:Ontology ;
  rdfs:label "DataChemist Core Ontology for Terminus DB"@en ;
  rdfs:comment "Core ontology defining the core predicate and classe building blocks that are used by the Terminus DB engine"@en ;
  dcog:rights "Copyright Data Chemist Ltd 2017-2019"@en ;
  dcog:author "Kevin C. Feeney"@en ;
  dcog:license <https://creativecommons.org/licenses/by-sa/2.0/>, <https://www.gnu.org/licenses/gpl-3.0.en.html> .

dcog:rights
  a owl:DatatypeProperty ;
  rdfs:range xsd:string ;
  rdfs:label "Rights"@en ;
  rdfs:comment "The statement of rights of the owner"@en .

dcog:author
  a owl:DatatypeProperty ;
  rdfs:range xsd:string ;
  rdfs:label "Author"@en ;
  rdfs:comment "The authors who developed the ontology"@en .

dcog:license
  a owl:ObjectProperty ;
  rdfs:range owl:Thing ;
  rdfs:label "License"@en ;
  rdfs:comment "The license governing the use of the resource"@en .

dcog:Tag
  a owl:Class ;
  dcog:tag dcog:abstract ;
  rdfs:label "Tag"@en ;
  rdfs:comment "Abstract class representing a tag that can be added to an element to qualify it"@en .

dcog:ClassTag
  a owl:Class ;
  rdfs:label "Class Tags"@en ;
  rdfs:subClassOf dcog:Enumerated, dcog:Tag ;
  rdfs:comment "Tags that can be added to classes to add meta information"@en ;
  owl:oneOf ( dcog:abstract ) .

dcog:abstract
  rdfs:label "Abstract"@en ;
  rdfs:comment "Indicates that the class is abstract - purely a logical construct, no base instantiations exist"@en ;
  a dcog:ClassTag .

dcog:Document
  a owl:Class ;
  dcog:tag dcog:abstract ;
  rdfs:label "Document Class"@en ;
  rdfs:comment "A class used to designate the primary data objects managed by the system - relationships and entities"@en .

dcog:Entity
  a owl:Class ;
  dcog:tag dcog:abstract ;
  rdfs:subClassOf dcog:Document ;
  rdfs:label "Entity Class"@en ;
  rdfs:comment "The class of entities (business objects / documents) managed by the system"@en .

dcog:Relationship
  a owl:Class ;
  rdfs:subClassOf dcog:Document ;
  dcog:tag dcog:abstract ;
  rdfs:label "Relationship"@en ;
  rdfs:comment "The class of relationship objects - documents which relate other entities together"@en .

dcog:Enumerated
  a owl:Class ;
  dcog:tag dcog:abstract ;
  rdfs:label "Enumerated Set"@en ;
  rdfs:comment "A class representing enumerated types / choice sets"@en .

dcog:TemporallyScoped
  a owl:Class ;
  dcog:tag dcog:abstract ;
  rdfs:comment "The class of things that are temporally scoped"@en ;
  rdfs:label "Temporally Scoped"@en .

dcog:GeographicallyScoped
  a owl:Class ;
  dcog:tag dcog:abstract ;
  rdfs:comment "The class of things that are geographically scoped"@en ;
  rdfs:label "Geographically Scoped"@en .

dcog:GeotemporallyScoped
  a owl:Class ;
  dcog:tag dcog:abstract ;
  rdfs:comment "The class of things that are geo-temporally scoped"@en ;
  rdfs:label "Geo Temporally Scoped"@en .

dcog:geography
  a owl:ObjectProperty ;
  rdfs:label "Geographic Scope"@en ;
  rdfs:comment "The geographic scope in which the associated data is considered to exist"@en ;
  rdfs:domain dcog:GeographicallyScoped ;
  rdfs:range dcog:GeographicScoping .

dcog:temporality
  a owl:ObjectProperty ;
  rdfs:label "Temporal Scope"@en ;
  rdfs:comment "The time-scope in which the associated data is considered to exist"@en ;
  rdfs:domain dcog:TemporallyScoped ;
  rdfs:range dcog:TemporalScoping .

dcog:geotemporality
  a owl:ObjectProperty ;
  rdfs:label "Geotemporal Scope"@en ;
  rdfs:comment "The geo-temporal scope in which the associated data is considered to exist"@en ;
  rdfs:domain dcog:GeotemporallyScoped ;
  rdfs:range dcog:GeotemporalScoping .

dcog:TemporalScoping
  a owl:Class ;
  dcog:tag dcog:abstract ;
  rdfs:label "Temporal Scoping"@en ;
  rdfs:comment "Class representing all types of temporal scoping"@en .

dcog:GeotemporalScoping
  a owl:Class ;
  dcog:tag dcog:abstract ;
  rdfs:label "Geotemporal Scoping"@en ;
  rdfs:comment "Class representing all types of geotemporal scoping"@en .

dcog:GeographicScoping
  a owl:Class ;
  dcog:tag dcog:abstract ;
  rdfs:label "Geographic Scoping"@en ;
  rdfs:comment "Class representing all types of geographic scoping"@en .

dcog:TimePoint
  a owl:Class ;
  rdfs:label "Point in Time"@en ;
  rdfs:comment "Class representing things that are associated with points in time"@en ;
  dcog:tag dcog:abstract ;
  rdfs:subClassOf dcog:TemporalScoping, dcog:SingleTimepoint .

dcog:TimeRange
  rdfs:label "Time Range"@en ;
  a owl:Class ;
  rdfs:comment "A Time Range that may have a start and an end time."@en ;
  dcog:tag dcog:abstract ;
  rdfs:subClassOf dcog:TemporalScoping, dcog:SingleRangeLimits .

dcog:start
  rdfs:label "Start"@en ;
  rdfs:comment "The start of a time range, when the associated data is considered to begin its existance"@en ;
  a owl:ObjectProperty ;
  rdfs:range dcog:TimePoint ;
  rdfs:domain dcog:TimeRange .

dcog:end
  rdfs:label "End"@en ;
  rdfs:comment "The end of a time range, when the associated data is considered to cease existance"@en ;
  a owl:ObjectProperty ;
  rdfs:range dcog:TimePoint ;
  rdfs:domain dcog:TimeRange .

dcog:SingleRangeLimits
  a owl:Restriction ;
  owl:onProperty dcog:start, dcog:end ;
  owl:maxCardinality "1"^^xsd:nonNegativeInteger ;
  rdfs:label "Single Range"@en ;
  rdfs:comment "Time ranges can have at most 1 start and 1 end"@en .

dcog:SingleTimepoint
  a owl:Restriction ;
  owl:cardinality "1"^^xsd:nonNegativeInteger ;
  rdfs:label "Single Time Point"@en ;
  rdfs:comment "Time Points have exactly one value"@en .

dcog:QualifiedByConfidence
  a owl:Class ;
  dcog:tag dcog:abstract ;
  rdfs:label "Qualified by Confidence"@en ;
  rdfs:comment "Class representing all objects that can have an associated confidence qualifier"@en .

dcog:QualifiedByConfidencePercentage
  a owl:Class ;
  dcog:tag dcog:abstract ;
  rdfs:label "Qualified By Confidence %"@en ;
  rdfs:comment "Signifies objects which can have a confidence value associated with them that is expressed as a demical precentage, 100 - 0"@en ;
  rdfs:subClassOf dcog:QualifiedByConfidence, dcog:SinglePercentageConfidence .

dcog:SinglePercentageConfidence
  a owl:Restriction ;
  owl:onProperty dcog:percent ;
  owl:maxCardinality "1"^^xsd:nonNegativeInteger ;
  rdfs:label "Single Percentage"@en ;
  rdfs:comment "Only one confidence percentage value allowed"@en .

dcog:percent
  rdfs:label "Confidence %"@en ;
  rdfs:comment "The confidence, expressed as a percentage probability, that the value us true"@en ;
  a owl:DatatypeProperty ;
  rdfs:domain dcog:QualifiedByConfidencePercentage ;
  rdfs:range xsd:decimal .

dcog:QualifiedByConfidenceTag
  a owl:Class ;
  dcog:tag dcog:abstract ;
  rdfs:label "Qualified By Confidence Tag"@en ;
  rdfs:comment "Signifies objects which can have a confidence value associated with them that is expressed as a semantic tag"@en ;
  rdfs:subClassOf dcog:QualifiedByConfidence .

dcog:confidence_tag
  rdfs:label "Confidence Tag"@en ;
  rdfs:comment "How certain is the data?"@en ;
  a owl:ObjectProperty ;
  rdfs:domain dcog:QualifiedByConfidenceTag ;
  rdfs:range dcog:ConfidenceTag .

dcog:ConfidenceTag
  rdfs:label "Content Tags"@en ;
  rdfs:comment "Tags that can be added to annotations to indicate confidence in the value of some piece data"@en ;
  a owl:Class ;
  rdfs:subClassOf dcog:Enumerated ;
  owl:oneOf (
   dcog:inferred
   dcog:disputed
   dcog:uncertain
   dcog:dubious
 ) .

dcog:inferred
  rdfs:label "Inferred"@en ;
  rdfs:comment "The value has been logically inferred from other evidence"@en ;
  a dcog:ConfidenceTag, dcog:ClassTag .

dcog:dubious
  rdfs:label "Dubious"@en ;
  rdfs:comment "The evidence suggests this value is dubious - there is low confidence in its truth"@en ;
  a dcog:ConfidenceTag .

dcog:disputed
  rdfs:label "Disputed"@en ;
  rdfs:comment "The evidence is disputed - some believe this data to be incorrect"@en ;
  a dcog:ConfidenceTag .

dcog:uncertain
  rdfs:label "Uncertain"@en ;
  rdfs:comment "The evidence has a high degree of uncertainty"@en ;
  a dcog:ConfidenceTag .

dcog:Annotation
  a owl:Class ;
  dcog:tag dcog:abstract ;
  rdfs:label "Annotation"@en ;
  rdfs:comment "An Annotation object is interpreted as qualifying or extending the value of the data it annotates"@en .

dcog:Provenance
  a owl:Class ;
  dcog:tag dcog:abstract ;
  rdfs:label "Provenance"@en ;
  rdfs:comment "A Provenance Object contains information about the provenance (source, origin, updates) of the object that it annotates"@en .

dcog:annotates
  a owl:ObjectProperty ;
  rdfs:subPropertyOf dcog:pseudo_property ;
  rdfs:label "Annotates"@en ;
  rdfs:comment "Generic Annotation Property - a special property that enables automatic interlinking between horizontally partitioned graphs"@en ;
  rdfs:domain dcog:Annotation, dcog:Provenance ;
  rdfs:range owl:Thing .

dcog:annotates_value
  a owl:DatatypeProperty ;
  rdfs:subPropertyOf dcog:pseudo_property ;
  rdfs:label "Annotates Value"@en ;
  rdfs:comment "The annotated value is considered to be qualified by this predicate. This enables annotations of specific datatype property values"@en ;
  rdfs:domain dcog:Annotation, dcog:Provenance ;
  rdfs:range xsd:anySimpleType .

dcog:pseudo_property
  a owl:ObjectProperty ;
  rdfs:label "Pseudeo Property"@en ;
  rdfs:comment "A pseudo property is an abstraction of a property that has a special significance for interlinking between documents in the schema"@en .

dcog:annotates_property
  a owl:DatatypeProperty ;
  rdfs:label "Annotates Property"@en ;
  rdfs:comment "The annotated property - with all its values - is considered to be qualified / extended by this predicate. This enables direct annotations on datatype properties"@en ;
  rdfs:subPropertyOf dcog:pseudo_property ;
  rdfs:domain dcog:Annotation, dcog:Provenance .

dcog:relationship_property
  a owl:ObjectProperty ;
  rdfs:label "Relationship Property"@en ;
  rdfs:domain dcog:Relationship ;
  rdfs:range owl:Thing;
  rdfs:comment "Used to identify the property of the relationship object that is specifically a source or target property"@en .

dcog:relationship_source
  a owl:ObjectProperty ;
  rdfs:label "Relationship Source"@en ;
  rdfs:comment "Signfies a property that points to the source of a relationship"@en ;
  rdfs:subPropertyOf dcog:relationship_property .

dcog:relationship_target
  a owl:ObjectProperty ;
  rdfs:label "Relationship Target"@en ;
  rdfs:comment "A Property that points to the target of a relationship"@en ;
  rdfs:subPropertyOf dcog:relationship_property .

