dcog:tag
  rdfs:label "Class Tag"@en ;
  rdfs:comment "Qualifies a class in the schema with a tag"@en ;
  rdfs:domain owl:Class;
  a owl:ObjectProperty ;
  rdfs:range dcog:ClassTag .

dcog:source_property
  a owl:ObjectProperty ;
  rdfs:label "Relationship Source"@en ;
  rdfs:comment "A special property of a relationship - the property that points to the relationship's source"@en ;
  rdfs:subPropertyOf dcog:pseudo_property .

dcog:target_property
  a owl:ObjectProperty ;
  rdfs:label "Relationship Target"@en ;
  rdfs:comment "A special property of a relationship - the property that points to the relationship's target"@en ;
  rdfs:subPropertyOf dcog:pseudo_property .

dcog:annotates
  a owl:ObjectProperty ;
  rdfs:subPropertyOf dcog:pseudo_property ;
  rdfs:label "Annotates"@en ;
  rdfs:comment "Generic Annotation Property - a special property that enables automatic interlinking between horizontally partitioned graphs"@en ;
  rdfs:domain dcog:Annotation, dcog:Provenance ;
  rdfs:range owl:Thing .

dcog:annotates_value
  a owl:DatatypeProperty ;
  rdfs:subPropertyOf dcog:pseudo_property ;
  rdfs:label "Annotates Value"@en ;
  rdfs:comment "The annotated value is considered to be qualified by this predicate. This enables annotations of specific datatype property values"@en ;
  rdfs:domain dcog:Annotation, dcog:Provenance ;
  rdfs:range xsd:anySimpleType .

dcog:pseudo_property
  a owl:ObjectProperty ;
  rdfs:label "Pseudeo Property"@en ;
  rdfs:comment "A pseudo property is an abstraction of a property that has a special significance for interlinking between documents in the schema"@en .

dcog:annotates_property
  a owl:DatatypeProperty ;
  rdfs:label "Annotates Property"@en ;
  rdfs:comment "The annotated property - with all its values - is considered to be qualified / extended by this predicate. This enables direct annotations on datatype properties"@en ;
  rdfs:subPropertyOf dcog:pseudo_property ;
  rdfs:domain dcog:Annotation, dcog:Provenance .

