@prefix rdfs: <http://www.w3.org/2000/01/rdf-schema#> .
@prefix xsd: <http://www.w3.org/2001/XMLSchema#> .
@prefix owl: <http://www.w3.org/2002/07/owl#> .
@prefix tcs: <http://terminusdb.com/schema/tcs#> .
@prefix xdd: <http://terminusdb.com/schema/xdd#> .
@prefix vio: <http://terminusdb.com/schema/vio#> .

<https://datachemist.net/ontology/vio>
  a owl:Ontology ;
  rdfs:label "Terminus Violations Schema"@en ;
  rdfs:comment "Schema describing all of the errors and violations that can be detected by the Terminus DB Engine and the structure of the documents produced"@en ;
  tcs:rights "Copyright Data Chemist Ltd. 2017-2019"@en ;
  tcs:author "Gavin Mendel-Gleason"@en, "Kevin C. Feeney"@en, "Kitty Jose"@en;
  tcs:license <https://creativecommons.org/licenses/by-sa/2.0/>, <https://www.gnu.org/licenses/gpl-3.0.en.html> .

vio:ViolationReport
  rdfs:label "Violation Report"@en ;
  rdfs:comment "A report of violations found in quality-testing of a document or graph fragment"@en ;
  a owl:Class ;
  rdfs:subClassOf tcs:Entity.

vio:InstanceDataViolationReport
  rdfs:label "Instance Data Violation Report"@en ;
  rdfs:comment "A report of violations of schema rules encountered in quality-testing of instance data"@en;
  a owl:Class ;
  rdfs:subClassOf tcs:Entity, vio:ViolationReport, vio:RestrictInstanceViolation .

vio:SchemaViolationReport
  rdfs:label "Schema Violation Report"@en ;
  rdfs:comment "A report of violations encountered in quality-testing of schema rules"@en;
  a owl:Class ;
  rdfs:subClassOf tcs:Entity, vio:ViolationReport, vio:RestrictSchemaViolation .

vio:violation
  rdfs:label "Violation"@en ;
  rdfs:comment "The set of violations that make up the violation report"@en ;
  a owl:ObjectProperty ;
  rdfs:domain vio:ViolationReport ;
  rdfs:range vio:Violation .  

vio:RestrictSchemaViolation
  a owl:Restriction ;
  rdfs:label "Schema Violation"@en;
  rdfs:comment "Restricts schema violation reports to only including schema violations"@en;
  owl:onProperty vio:violation ;
  owl:allValuesFrom vio:SchemaViolation.

vio:RestrictInstanceViolation
  a owl:Restriction ;
  rdfs:label "Insgtance Data Violation"@en;
  rdfs:comment "Restricts Instance Data violation reports to only including instance data violations"@en;
  owl:onProperty vio:violation ;
  owl:allValuesFrom vio:InstanceDataViolation.

vio:Violation
  rdfs:label "Violation"@en ;
  tcs:tag tcs:abstract;
  rdfs:comment "A specific violation of a reasoning rule"@en ;
  rdfs:subClassOf vio:MessageCardinalityRestriction;
  a owl:Class .

vio:message
  rdfs:label "Message"@en ;
  rdfs:comment "The textual message to the user explaining the violation - every violation has an associated message"@en ;
  a owl:DatatypeProperty ;
  rdfs:domain vio:Violation ;
  rdfs:range xsd:string .

vio:MessageCardinalityRestriction
  owl:cardinality "1"^^xsd:nonNegativeInteger ;
  rdfs:label "Mandatory Unique Message"@en;
  rdfs:comment "Every violation contains exactly one message string"@en;
  a owl:Restriction ;
  owl:onProperty vio:message .
  
vio:SchemaViolation
  tcs:tag tcs:abstract;
  rdfs:label "Schema Violation"@en ;
  rdfs:comment "A Violation of the rules relating to valid schema definition. 
  Schema violations indicate an attempt to change a schema into an invalid state 
  - a situation where prevention is always much better than cure!"@en ;
  a owl:Class ;
  rdfs:subClassOf vio:Violation .

vio:ClassViolation
  tcs:tag tcs:abstract;
  rdfs:label "Class Violation"@en ;
  rdfs:comment "A violation that relates to a class definition in the schema"@en;
  a owl:Class ;
  rdfs:subClassOf vio:ClassCardinalityRestriction, vio:SchemaViolation .

vio:class
  rdfs:label "Class"@en ;
  rdfs:comment "The specific class whose definition contains the violation"@en ;
  a owl:DatatypeProperty ;
  rdfs:domain vio:ClassViolation ;
  rdfs:range xsd:string .

vio:ClassCardinalityRestriction
  a owl:Restriction ;
  rdfs:label "Mandatory Class"@en;
  rdfs:comment "Every class violation is associated with exactly one class"@en;
  owl:cardinality "1"^^xsd:nonNegativeInteger ;
  owl:onProperty vio:class .

vio:DuplicateClassLabelViolation
  rdfs:label "Duplicate Class Label Violation"@en ;
  rdfs:comment "The class should have a single, unique label in any language"@en ;
  a owl:Class ;
  rdfs:subClassOf vio:ClassViolation .

vio:InvalidClassViolation
  rdfs:label "Invalid Class Violation"@en ;
  rdfs:comment "A class referred to is not defined or is invalid"@en ;
  a owl:Class ;
  rdfs:subClassOf vio:ClassViolation .

vio:ClassInheritanceVioltion
  rdfs:label "Class Inheritance Violation"@en ;
  rdfs:comment "The violation is related to class inheritance"@en ;
  a owl:Class ;
  rdfs:subClassOf vio:ClassViolation, vio:ViolationWithParent, vio:ParentCardinalityRestriction.

vio:ViolationWithParent
 a owl:Class;
 rdfs:label "Violation with Parent"@en;
 rdfs:comment "A violation which relates to the parent of a class or instance"@en;
 tcs:tag tcs:abstract.

vio:parent
  rdfs:label "Parent Class"@en ;
  rdfs:comment "The parent class related to the violation"@en ;
  a owl:DatatypeProperty ;
  rdfs:domain vio:ViolationWithParent ;
  rdfs:range xsd:string .

vio:ParentCardinalityRestriction
  a owl:Restriction ;
  rdfs:label "Mandatory Parent"@en;
  rdfs:comment "Every class inheritance violation is associated with exactly one parent class"@en;
  owl:cardinality "1"^^xsd:nonNegativeInteger ;
  owl:onProperty vio:parent.

vio:InvalidIntersectionViolation
  rdfs:label "Invalid Intersection Violation"@en ;
  rdfs:comment "The class is defined as an intersection including an invalid class"@en ;
  a owl:Class ;
  rdfs:subClassOf vio:ClassInheritanceVioltion .

vio:InvalidParentViolation
  rdfs:label "Invalid Parent Violation"@en ;
  rdfs:comment "The parent class is not a valid class"@en ;
  a owl:Class ;
  rdfs:subClassOf vio:ClassInheritanceVioltion .

vio:InvalidUnionViolation
  rdfs:label "Invalid Union Violation"@en ;
  rdfs:comment "The class is defined as a union that includes an invalid class"@en ;
  a owl:Class ;
  rdfs:subClassOf vio:ClassInheritanceVioltion .

vio:ClassCycle
  rdfs:label "Class Cycle"@en ;
  rdfs:comment "A cyclical inheritance pattern"@en ;
  a owl:Class ;
  rdfs:subClassOf vio:ClassViolation .

vio:path
  rdfs:label "Path"@en ;
  rdfs:comment "The path that amounts to a cycle in the class inheritance hierarchy"@en ;
  a owl:ObjectProperty ;
  rdfs:domain vio:ClassCycle ;
  rdfs:range vio:ListEntry .

vio:ListEntry
  rdfs:label "List Entry"@en ;
  rdfs:comment "An entry in a list of paths"@en ;
  a owl:Class ;
  rdfs:subClassOf vio:IndexCardinalityRestriction, vio:PathComponentCardinalityRestriction .
  
vio:index
  rdfs:label "Index"@en ;
  rdfs:comment "The position in the inheritance cycle chain"@en ;
  a owl:DatatypeProperty ;
  rdfs:domain vio:ListEntry ;
  rdfs:range xsd:nonNegativeInteger .

vio:IndexCardinalityRestriction
  owl:maxCardinality "1"^^xsd:nonNegativeInteger ;
  a owl:Restriction ;
  rdfs:label "Single Mandatory Index"@en;
  rdfs:comment "Every List Entry in an inheritance must have a single index"@en;  
  owl:onProperty vio:index .

vio:path_component
  rdfs:label "Path Component"@en ;
  rdfs:comment "The particular class in this step in the inheritance cycle chain"@en ;
  a owl:DatatypeProperty ;
  rdfs:domain vio:ListEntry ;
  rdfs:range xsd:string.

vio:PathComponentCardinalityRestriction
  owl:cardinality "1"^^xsd:nonNegativeInteger ;
  a owl:Restriction ;
  rdfs:label "Single Mandatory Class"@en;
  rdfs:comment "Every List Entry in an inheritance must have a single class component"@en;  
  owl:onProperty vio:path_component .

vio:PropertyViolation
  rdfs:label "Property Violation"@en ;
  a owl:Class ;
  tcs:tag tcs:abstract;
  rdfs:comment "A violation that relates to a property definition in the schema"@en;
  rdfs:subClassOf vio:PropertyCardinalityRestriction, vio:SchemaViolation .

vio:property
  rdfs:label "Property"@en ;
  rdfs:comment "The property in which the specification error is found"@en ;
  a owl:DatatypeProperty ;
  rdfs:domain vio:PropertyViolation ;
  rdfs:range xsd:string .

vio:PropertyCardinalityRestriction
  owl:cardinality "1"^^xsd:nonNegativeInteger ;
  a owl:Restriction ;
  rdfs:label "Mandatory Property"@en;
  rdfs:comment "Every property violation is associated with exactly one property"@en;
  owl:onProperty vio:property .

vio:NonUniquePropertyName
  rdfs:label "Non Unique Property Name"@en ;
  rdfs:comment "Property Names must be unique"@en ;
  a owl:Class ;
  rdfs:subClassOf vio:PropertyViolation .

vio:DuplicatePropertyLabelViolation
  rdfs:label "Duplicate Property Label Violation"@en ;
  rdfs:comment "The property should have a unique label"@en ;
  a owl:Class ;
  rdfs:subClassOf vio:PropertyViolation .

vio:PropertyTypeOverload
  rdfs:label "Property Type Overload"@en ;
  rdfs:comment "The property is defined as both an object property and a datatype property"@en ;
  a owl:Class ;
  rdfs:subClassOf vio:PropertyViolation .

vio:PropertyInheritanceViolation
  rdfs:label "Property Inheritance Violation"@en ;
  rdfs:comment "A violation that relates to property inheritance"@en ;
  a owl:Class ;
  tcs:tag tcs:abstract ;
  rdfs:subClassOf vio:PropertyViolation, vio:ParentPropertyCardinalityRestriction .
  
vio:parent_property
  rdfs:label "Parent Property"@en ;
  rdfs:comment "The parent property that is associated with the violation"@en ;
  a owl:DatatypeProperty ;
  rdfs:domain vio:PropertyInheritanceViolation ;
  rdfs:range xsd:string.

vio:ParentPropertyCardinalityRestriction
  owl:cardinality "1"^^xsd:nonNegativeInteger ;
  a owl:Restriction ;
  rdfs:label "Mandatory Parent Property"@en;
  rdfs:comment "Every inherticance property violation is associated with exactly one parent property"@en;
  owl:onProperty vio:parent_property .

vio:OrphanPropertyViolation
  rdfs:label "Orphan Property Violation"@en ;
  rdfs:comment "The property inherits from an undefined property"@en ;
  a owl:Class ;
  rdfs:subClassOf vio:PropertyInheritanceViolation .

vio:UntypedPropertyViolation
  rdfs:label "Untyped Property Violation"@en ;
  rdfs:comment "The property does not have a valid definition that enables it to be identified as either a datatype or an object property"@en ;
  a owl:Class ;
  rdfs:subClassOf vio:PropertyViolation .

vio:UntypedPropertyWithDomain
  rdfs:label "Untyped Property With Domain"@en ;
  rdfs:comment "A property that is specified as having a domain but has no valid definition or type"@en ;
  a owl:Class ;
  rdfs:subClassOf vio:UntypedPropertyViolation .

vio:domain
  rdfs:label "Domain"@en ;
  rdfs:comment "The class that is defined as being the domain of the invalid property"@en ;
  a owl:DatatypeProperty ;
  rdfs:domain vio:UntypedPropertyWithDomain ;
  rdfs:range xsd:string .

vio:UntypedPropertyWithRange
  rdfs:label "Untyped Property With Range"@en ;
  rdfs:comment "A property that is specified as having a range but has no valid definition or type"@en ;
  a owl:Class ;
  rdfs:subClassOf vio:UntypedPropertyViolation .

vio:range
  rdfs:label "Range"@en ;
  rdfs:comment "The class that is the defined as being the range of the invalid property"@en ;
  a owl:DatatypeProperty ;
  rdfs:domain vio:UntypedPropertyWithRange ;
  rdfs:range xsd:string.

vio:UntypedPropertyWithParent
  rdfs:label "Untyped Property with Parent"@en ;
  rdfs:comment "A property that is specified as having a parent property but has no defined type"@en ;
  a owl:Class ;
  rdfs:subClassOf vio:PropertyInheritanceViolation, vio:UntypedPropertyViolation .

vio:PropertyDomainNotSubsumed
  rdfs:label "Property Domain Not Subsumed"@en ;
  rdfs:comment "The property has a domain but the domain is not subsumed by the parent domain"@en ;
  a owl:Class ;
  rdfs:subClassOf vio:ClassInheritanceVioltion, vio:PropertyInheritanceViolation .

vio:PropertyRangeNotSubsumed
  rdfs:label "Property Range Not Subsumed"@en ;
  a owl:Class ;
  rdfs:comment "The property has a range but that range is not subsumed by the range of the parent property"@en;
  rdfs:subClassOf vio:ClassInheritanceVioltion, vio:PropertyInheritanceViolation .

vio:InvalidClassInProperty
  rdfs:label "Invalid Class in Property"@en ;
  rdfs:comment "An invalid class is referred to in a property definition"@en ;
  a owl:Class ;
  rdfs:subClassOf vio:InvalidClassViolation, vio:PropertyViolation .

vio:InvalidClassInDomain
  rdfs:label "Invalid Class in Domain"@en ;
  rdfs:comment "The domain of a property refers to an invalid class"@en ;
  a owl:Class ;
  rdfs:subClassOf vio:InvalidClassInProperty .

vio:InvalidClassInRange
  rdfs:label "Invalid Class in Range"@en ;
  rdfs:comment "A class referred to in a range is invalid"@en ;
  a owl:Class ;
  rdfs:subClassOf vio:InvalidClassInProperty .

vio:InstanceDataViolation
  rdfs:label "Instance Violation"@en ;
  rdfs:comment "A Violation of the rules defined in the schema, related to instance data. 
  Instance Data violations indicate situations where the data does not conform to the rules defined in the schema"@en ;
  a owl:Class ;
  tcs:tag tcs:abstract ;
  rdfs:subClassOf vio:Violation .

vio:ViolationWithSubject
  rdfs:label "Violation with Subject"@en ;
  rdfs:comment "An instance data violation that is related to a specific subject (ID / URL) element"@en ;
  a owl:Class ;
  rdfs:subClassOf vio:InstanceDataViolation .

vio:subject
  rdfs:label "Subject"@en ;
  rdfs:comment "The subject of the triple that relates to the violation"@en ;
  a owl:DatatypeProperty ;
  rdfs:domain vio:ViolationWithSubject ;
  rdfs:range xsd:string .

vio:ViolationWithPredicate
  rdfs:label "Violation with Predicate"@en ;
  rdfs:comment "An instance data violation that is associated with a particular predicate encountered in the data."@en ;
  a owl:Class ;
  rdfs:subClassOf vio:InstanceDataViolation .
 
vio:predicate
  rdfs:label "Predicate"@en ;
  rdfs:comment "The relevant predicate in a violation"@en ;
  a owl:DatatypeProperty ;
  rdfs:domain vio:ViolationWithPredicate ;
  rdfs:range xsd:string .

vio:CardinalityViolation
  rdfs:label "Cardinality Violation"@en ;
  rdfs:comment "An instance data violation of a cardinality rule (cardinality rules apply to subject / predicate combinations)"@en ;
  a owl:Class ;
  rdfs:subClassOf vio:ViolationWithSubject, vio:ViolationWithPredicate .

vio:ViolationWithObject
  rdfs:label "Violation with Object"@en ;
  rdfs:comment "An instance data violation that is associated with a particular object"@en ;
  a owl:Class ;
  rdfs:subClassOf vio:InstanceDataViolation .

vio:object
  rdfs:label "Object ID"@en ;
  rdfs:comment "The object ID (URL) relevant to the violation"@en ;
  a owl:DatatypeProperty ;
  rdfs:domain vio:ViolationWithObject ;
  rdfs:range xsd:string .

vio:ViolationWithDatatypeObject
  rdfs:label "Violation with Datatype Object"@en ;
  rdfs:comment "An instance data violation that is associated with a particular literal value"@en ;
  a owl:Class ;
  rdfs:subClassOf vio:InstanceDataViolation .

vio:literal
  rdfs:label "Literal Value"@en ;
  rdfs:comment "The datatype object / literal related to the violation"@en ;
  a owl:DatatypeProperty ;
  rdfs:domain vio:ViolationWithDatatypeObject ;
  rdfs:range xsd:anySimpleType.

vio:DatatypeSubsumptionViolation
  rdfs:label "Datatype Subsumption Violation"@en ;
  rdfs:comment "The datatype parent has a violation"@en ;
  a owl:Class ;
  rdfs:subClassOf vio:ViolationWithDatatypeObject .
  
vio:parent_type
  rdfs:label "Parent Type"@en ;
  rdfs:comment "Subsuming Type"@en ;
  a owl:DatatypeProperty ;
  rdfs:domain vio:DatatypeSubsumptionViolation ;
  rdfs:range xsd:string .

vio:base_type
  rdfs:label "Base Type"@en ;
  rdfs:comment "Subsumed Type"@en ;
  a owl:DatatypeProperty ;
  rdfs:domain vio:ViolationWithDatatypeObject ;
  rdfs:range xsd:string .


 vio:PropertyCycleViolation 
   rdfs:label "Property Cycle"@en ;
   rdfs:comment "A cycle in a property inheritance hierarchy"@en ;
   a owl:Class.
   
vio:UntypedInstance
   rdfs:label "Untyped Instance"@en;
   rdfs:comment "A subject is used without a rdf:type being defined for it"@en. 
   a owl:Class;
   rdfs:subClassOf vio:ViolationWithSubject.

vio:InstanceSubsumptionViolation      
   rdfs:label "Instance Subsumption Violation"@en;
   rdfs:comment "An instance subject has an invalid parent"@en. 
   a owl:Class;
   rdfs:subClassOf vio:ViolationWithSubject, vio:ViolationWithParent.

